\documentclass{article}
% ‡@ ‡A ‡B

\def\AHM{\mathrm{AHM}}

\begin{document}
\def\LEM{\mathrm{LEM}}

$$
\LEM(X,Y)=\exp\left(\frac{\log X+\log Y}{2}\right),
$$


$$
A_0=X\succ 0
$$

$$
H_0=Y\succ 0
$$

\begin{eqnarray*}
A_{t+1} &=& \frac{A_t+H_t}{2}\\
H_{t+1} &=& 2\, (A_t^{-1}+H_t^{-1})^{-1} 
\end{eqnarray*}
 $$
\AHM(X,Y)=\lim_{t\rightarrow +\infty} A_t=\lim_{t\rightarrow +\infty} H_t =X^{\frac{1}{2}}\, (X^{-\frac{1}{2}}\, Y\, X^{-\frac{1}{2}})^{\frac{1}{2}}\, X^{\frac{1}{2}}=G(X,Y)
$$

$GX^{-1}G=Y$


$$
M=\frac{1}{2} M\#_p X + \frac{1}{2}  M\#_p Y
$$


$$
m=\frac{1}{2} m^{1-p}x^p + \frac{1}{2} m^{1-p}y^p
$$
$$
m=\left(\frac{1}{2}x^p+\frac{1}{2}y^p\right)^{\frac{1}{p}}=M_p(x,y)
$$

$$
X\#_t Y= 
X^{\frac{1}{2}}\, \left(X^{-\frac{1}{2}}\, Y\, X^{-\frac{1}{2}}\right)^t\, X^{\frac{1}{2}},
$$

$$
\lim_{p\rightarrow 0}M_p(x,y)=G(x,y)
$$


$$
M=\frac{1}{2} M\#_p X + \frac{1}{2}  M\#_p Y
$$

$M(X,Y)$ is said operator monotone~\cite{bhatia2006riemannian} if for $X'\preceq X$ and $Y'\preceq Y$, we have
$M(X',Y')\preceq M(X,Y)$.

\end{document}

$$
a_0=x>0, h_0=y>0
$$

 
\begin{eqnarray*}
a_{t+1} &=& A(a_t,h_t)=\frac{a_t+h_t}{2},\\
h_{t+1} &=& H(a_t,h_t)=\frac{2a_th_t}{a_t+h_t},
\end{eqnarray*}
 

$$
\AHM(x,y)=\lim_{t\rightarrow\infty} a_t=\lim_{t\rightarrow\infty} h_t=\sqrt{xy}=G(x,y)
$$

$$
x=r_1\, e^{i\theta_1}, y=r_2\, e^{i\theta_2}
$$  

 

$$
\AHM(x,y)=\lim_{t\rightarrow\infty} a_t=\lim_{t\rightarrow\infty} h_t= \AHM(z_1,z_2)=\sqrt{r_1r_2}\, e^{i\frac{\theta_1+\theta_2}{2}}=G(r_1,r_2)e^{i A(\theta_1,\theta_2)}
$$


$$
A_0=X\succ 0, h_0=Y\succ 0
$$
\begin{eqnarray*}
A_{t+1} &=& \frac{A_t+H_t}{2}\\
H_{t+1} &=& 2\, (A_t^{-1}+H_t^{-1})^{-1} 
\end{eqnarray*}
 $$
\AHM(X,Y)=\lim_{t\rightarrow +\infty} A_t=\lim_{t\rightarrow +\infty} H_t =X^{\frac{1}{2}}\, (X^{-\frac{1}{2}}\, Y\, X^{-\frac{1}{2}})^{\frac{1}{2}}\, X^{\frac{1}{2}}=G(X,Y)
$$






\end{document}